

Integrating both sides, we get

$$xe^{-\frac{1}{y}} = \int \frac{1}{y^3} e^{-\frac{1}{y}} dy + C = -\int ze^z dz + C, \text{ where } z = -\frac{1}{y}$$

$$= -(z-1)e^z + C = \left(\frac{1}{y} + 1\right) e^{-\frac{1}{y}} + C$$

$$\text{or, } x = \left(\frac{1}{y} + 1\right) + Ce^{\frac{1}{y}}.$$

11. Solve the equation:  $(1+y^2)dx - (\tan^{-1}y - x)dy = 0$ .

*Solution*

We rewrite the equation as

$$\frac{dx}{dy} + \frac{x}{1+y^2} = \frac{\tan^{-1}y}{1+y^2}.$$

This is a linear differential equation, whose integrating factor is

$$e^{\int \frac{dy}{1+y^2}} = e^{\tan^{-1}y}.$$

Multiplying the equation by  $e^{\tan^{-1}y}$ , we get

$$\left(\frac{dx}{dy} + \frac{x}{1+y^2}\right) e^{\tan^{-1}y} = \frac{\tan^{-1}y}{1+y^2} e^{\tan^{-1}y} \quad \text{or, } \frac{d}{dy}(xe^{\tan^{-1}y}) = \frac{\tan^{-1}y}{1+y^2} e^{\tan^{-1}y}.$$

Integrating both sides, we get

$$xe^{\tan^{-1}y} = \int \frac{\tan^{-1}y}{1+y^2} e^{\tan^{-1}y} dy = \int ze^z dz, \text{ where } z = \tan^{-1}y$$

$$= (z-1)e^z + C = (\tan^{-1}y - 1)e^{\tan^{-1}y} + C$$

$$\text{or, } x = \tan^{-1}y - 1 + Ce^{-\tan^{-1}y}.$$

12. Solve the equation:  $\frac{dy}{dx} + \frac{y}{\sqrt{(1-x^2)^3}} = \frac{x + \sqrt{1-x^2}}{(1-x^2)^2}$ .

*Solution*

The given equation is a linear differential equation whose integrating factor is

$$e^{\int \frac{dx}{\sqrt{(1-x^2)^3}}} = e^{\int \sec^2 \theta d\theta}, \text{ where } x = \sin \theta$$

$$= e^{\tan \theta} = e^{\frac{x}{\sqrt{1-x^2}}}.$$

Multiplying the given equation by  $e^{\frac{x}{\sqrt{1-x^2}}}$ , we get

$$\left( \frac{dy}{dx} + \frac{y}{\sqrt{(1-x^2)^3}} \right) e^{\frac{x}{\sqrt{1-x^2}}} = \frac{x + \sqrt{1-x^2}}{(1-x^2)^2} e^{\frac{x}{\sqrt{1-x^2}}}$$

or, 
$$\frac{d}{dx} \left( y e^{\frac{x}{\sqrt{1-x^2}}} \right) = \frac{x + \sqrt{1-x^2}}{(1-x^2)^2} e^{\frac{x}{\sqrt{1-x^2}}}$$

Integrating, we get

$$\begin{aligned} y e^{\frac{x}{\sqrt{1-x^2}}} &= \int \frac{x + \sqrt{1-x^2}}{(1-x^2)^2} e^{\frac{x}{\sqrt{1-x^2}}} dx \\ &= \int \frac{\sin \theta + \cos \theta}{\cos^3 \theta} e^{\tan \theta} d\theta, \text{ where } x = \tan \theta \\ &= \int (1+z) e^z dz, \text{ where } z = \tan \theta \\ &= z e^z + C = \tan \theta e^{\tan \theta} + C \\ &= \frac{x}{\sqrt{1-x^2}} e^{\frac{x}{\sqrt{1-x^2}}} + C \end{aligned}$$

or, 
$$y = \frac{x}{\sqrt{1-x^2}} + C e^{-\frac{x}{\sqrt{1-x^2}}}$$

13. Solve the equation:  $\frac{dy}{dx} + (2x \tan^{-1} y - x^3)(1+y^2) = 0$ .

**Solution**

We rewrite the equation as

$$\frac{dy}{dx} + 2x \tan^{-1} y (1+y^2) = x^3 (1+y^2)$$

Dividing  $1+y^2$ , we get

$$\frac{1}{1+y^2} \frac{dy}{dx} + 2x \tan^{-1} y = x^3$$

Putting  $z = \tan^{-1} y$ , we get

$$\frac{dz}{dx} + 2xz = x^3$$

This is a linear differential equation whose integrating factor is

$$e^{\int 2x dx} = e^{x^2}$$



42.  $[1 + x(1 + y^2)]dy + y(1 + y^2)dx = 0,$
43.  $y \ln y dx + (x - \ln y)dy = 0,$
44.  $\sin 2x \frac{dy}{dx} = y + \tan x,$
45.  $dx + xdy = e^{-y} \sec^2 y dy,$
46.  $(x^2 y^3 + 2xy)dy = dx,$
47.  $(x + 2y^3) \frac{dy}{dx} = y,$
48.  $\frac{dy}{dx} + \frac{1}{x} = \frac{e^y}{x^2},$
- ~~49.~~  $\frac{dy}{dx} - \frac{\tan y}{1+x} = (1+x)e^x \sec y,$
50.  $\frac{dy}{dx} + \frac{y \ln y}{x} = \frac{y(\ln y)^2}{x^2},$
- ~~51.~~  $\frac{dy}{dx} + \frac{xy}{1-x^2} = x\sqrt{y},$
- ~~52.~~  $\sin x \frac{dy}{dx} - y \cos x + y^2 = 0,$
53.  $xy - \frac{dy}{dx} = y^3 e^{-x^2},$
- ~~54.~~  $\frac{dz}{dx} + \frac{z}{x} \ln z = \frac{z(\ln z)^2}{x^2},$
- ~~55.~~  $x \frac{dy}{dx} + 3y = x^3 y^2,$
- ~~56.~~  $(xy + x^3 y^3) \frac{dy}{dx} = 1,$

[Hints: Rewrite the equation as  $\frac{1}{x^3} \frac{dx}{dy} - \frac{y}{x^2} = y^3$  and put  $z = \frac{1}{x^2}$ ]

57.  $(x^2 + y^2 + 2y)dy + 2xdx = 0,$
58.  $y(2xy + e^x)dx - e^x dy = 0,$
59. Show that the general solution of the equation

$$\frac{dy}{dx} + P(x)y = Q(x)$$

can be written in the form  $y = k(u - v) + v$ , where  $k$  is a constant and  $u, v$  are two particular solutions of the equation.

[Hints: If  $u, v$  are two particular solutions of the equation, then any linear combination of these, say  $y = au + bv$ , where  $a, b$  are arbitrary constants, will be a general solution of the given equation. Choosing  $a = k, b = 1 - k$ , we see that

$$y = ku + (1 - k)v = k(u - v) + v$$

is a general solution of the given equation.]

60. Show that the solution of the equation

$$\frac{dy}{dx} + P(x)y = Q(x)$$

can be put in the form

$$y = \frac{Q}{P} - e^{-\int P dx} \left[ \int e^{\int P dx} d\left(\frac{Q}{P}\right) + C \right].$$

[Hints: Let  $z = y - \frac{Q}{P}$ , then  $\frac{dz}{dx} = \frac{dy}{dx} - \frac{d}{dx}\left(\frac{Q}{P}\right).$

Multiplying the above equation by  $e^{x^2}$ , we get

$$\left(\frac{dz}{dx} + 2xz\right)e^{x^2} = x^3e^{x^2} \quad \text{or,} \quad \frac{d}{dx}(ze^{x^2}) = x^3e^{x^2}.$$

Integrating both sides, we get

$$ze^{x^2} = \int x^3e^{x^2} dx + C$$

$$= \frac{1}{2} \int ue^u du + C, \text{ where } u = x^2$$

$$= \frac{1}{2}(u-1)e^u + C = \frac{1}{2}(x^2-1)e^{x^2} + C$$

$$\text{or,} \quad \tan^{-1} y = \frac{1}{2}(x^2-1) + Ce^{-x^2}.$$

14. Solve the equation:  $\frac{dy}{dx} = y^2 + \frac{1}{2x^2}$ .

*Solution*

$$\frac{dy}{dx} = y^2 + \frac{1}{2x^2}$$

$$\frac{dy}{dx} = \frac{2x^2y^2 + 1}{2x^2} \quad x \frac{dy}{dx} + y = \frac{2x^2y^2 + 1}{2x} + y = \frac{2x^2y^2 + 2xy + 1}{2x}$$

$$\Rightarrow d(xy) = \frac{1 + (1 + 2xy)^2}{4x} dx \Rightarrow d(2xy + 1) = \frac{1 + (1 + 2xy)^2}{2x} dx$$

$$\frac{d(2xy + 1)}{1 + (1 + 2xy)^2} = \frac{dx}{2x}.$$

Integrating, we get

$$\tan^{-1}(1 + 2xy) = \frac{1}{2} \ln x + C.$$

15. Show that in an equation of the form  $yf(xy)dx + xg(xy)dy = 0$  the variables can be separated by the substitution  $xy = v$ . Hence find the solution of the equation

$$(x^3y^3 + x^2y^2 + xy + 1)ydx + (x^3y^3 - x^2y^2 - xy + 1)xdy = 0.$$

*Solution*

Putting  $xy = v$ , i.e.,  $x \frac{dy}{dx} + y = \frac{dv}{dx}$  in the given equation, we get

$$yf(v) + g(v) \left[ \frac{dv}{dx} - y \right] = 0$$

$$\text{or, } y[f(v) - g(v)] + g(v) \frac{dv}{dx} = 0 \quad \text{or, } \frac{g(v)dv}{v[f(v) - g(v)]} + \frac{dx}{x} = 0.$$

- (b) Find a solution of the differential equation

$$\frac{dy}{dx} - y \tan x = 0$$

in the form  $y = y_1(x)$ , say. Hence solve

$$\frac{dy}{dx} - y \tan x = \cos x$$

by the substitution  $y = y_1(x)v(x)$ .

[C.H. 1990]

- (c) When  $P$  and  $Q$  are functions of  $x$  alone or constants, solve:

(i)  $\frac{dy}{dx} + Py = Q$  and (ii)  $\frac{dy}{dx} + Py = Qy^n$ . [C.H. 1990]

2. Solve by the method of variation of parameters (i.e., accepting a solution of reduced equation):

(a)  $\frac{dy}{dx} - 5y = \sin x$ .

(b)  $\frac{dy}{dx} + 6y = 18e^{3x}$ .

(c)  $\frac{dx}{dt} + \frac{1}{t}x = t^2$ .

(d)  $\frac{dy}{dt} + e^t y = e^t$ .

3. (a)  $\frac{dy}{dx} + y \cot x = 2 \cos x$ .

(b)  $\frac{dy}{dx} + \frac{1-2x}{x^2}y = 1$ .

4. (a)  $(1-x^2) \frac{dy}{dx} - xy = 1$ .

(b)  $\frac{dy}{dx} + \frac{y}{(1-x^2)^{3/2}} = \frac{x + \sqrt{1-x^2}}{(1-x^2)^2}$ .

5. (a)  $\frac{dy}{dx} + \frac{y}{x} = \frac{1}{x^2}$ .

(b)  $\frac{dy}{dx} + \frac{4x}{x^2+1}y = \frac{1}{(x^2+1)^2}$ .

(a)  $x \cos x \frac{dy}{dx} + (x \sin x + \cos x)y = 1$ .

(b)  $y^2 + \left(x - \frac{1}{y}\right) \frac{dy}{dx} = 0$ .

(a)  $x(1-x^2) \frac{dy}{dx} + (2x^2-1)y = ax^3$ .

[C.H. 1990]

8.  $\sqrt{a^2+x^2} \frac{dy}{dx} + y = \sqrt{a^2+x^2} - x$ .

9.  $\frac{dy}{dx} - \frac{2y}{x+1} = (x+1)^{\frac{3}{2}}$ .

10.  $a \frac{du}{d\theta} + u(\tan \theta)u = \tan \theta$ .

11.  $(x+a) \frac{dy}{dx} - 3y = (x+a)^2$ .

12.  $x \log x \frac{dy}{dx} + y = 2 \log x$ .

13.  $(x+y+1) dy = dx$ .

14.  $(1+y^2) dx = (\tan^{-1} y - x) dy$ .

15.  $2(1-xy) \frac{dy}{dx} = y^2$ .

16.  $(x+2y^2) \frac{dy}{dx} = y$ .

17.  $\frac{dy}{dx} + \frac{1}{x}y = x^2 y^3$ .

18.  $\frac{dy}{dx} + \frac{x}{1-x^2}y = x\sqrt{y}$ .

19. (a)  $3 \frac{dy}{dx} + \frac{2}{x+1}y = \frac{x^2}{y^2}$ .

(b)  $x \frac{dy}{dx} + y = xy^2$ .

[C.H. 1980]

20. (a)  $3x(1-x^2) y^3 \frac{dy}{dx} + (2x^2-1)y^3 = ax^3$ .

(b)  $2x^2 \frac{dy}{dx} = xy + y^2$ .

[C.H. 1983]

21.  $x \frac{dy}{dx} + y = y^2 \log x$ .

[C.H. 1993]

22.  $\sec^2 y \frac{dy}{dx} + 2x \tan y = x^2$ .

[C.H. 1984]

23.  $x \frac{dy}{dx} + y = y^3 x^2 \cos x$ .

24.  $dx + x dy = e^{-y} \sec^3 y dy$ .

25.  $(x^2 y^3 + xy) dy = dx$ .

26.  $(x^2 y^3 + 2xy) dy = dx$ .

[C.H. 1985, '95]

Of Eqn-8